src/lifting.v
@@ -5,26 +5,37 @@ From iris_simp_lang Require Import stack_ra implang imp_notation lifting_expr.
 Section wp.
 
 Context `{!gen_heapGS loc val Σ} `{!envGS val Σ} `{!invGS_gen HasNoLc Σ}.
+Variable (F : func_env).
 
 Implicit Types (ρ : @env_state val) (σ : gmap loc val).
 
-Definition wp_pre (wp : func_env -d> coPset -d> stmt -d> assert -d> assert) :
-    func_env -d> coPset -d> stmt -d> assert -d> assert := λ F E s Q,
- (∀ σ ρ, state_interp σ ρ ={E,∅}=∗ ∀ r, env_match ρ r -∗ ∃ s' r' σ' stk stk',
-        ⌜step F s (Build_state r σ stk) s' (Build_state r' σ' stk')⌝ ∗
-        ▷ |={∅,E}=> ∃ ρ', state_interp σ' ρ' ∗ env_match ρ' r' ∗ wp F E s' Q)%I.
+Fixpoint make_stack (k : stack) : env_state * nat :=
+  match k with
+  | [] => (∅, O)
+  | (r, _) :: k' => let '(ρ, n) := make_stack k' in (<[n := r]>ρ, S n)
+  end.
+
+Definition stack_match ρ r k := assert_of (λ n, ⌜let '(ρ0, n0) := make_stack k in n = n0 ∧ ρ = <[n := r]>ρ0⌝)%I.
+
+Definition wp_pre (wp : coPset -d> stmt -d> assert -d> assert) :
+    coPset -d> stmt -d> assert -d> assert := λ E s Q,
+ (∀ σ ρ, state_interp σ ρ ={E,∅}=∗ ∀ r k, stack_match ρ r k -∗ ∃ s' r' σ' k',
+        ⌜step F s (Build_state r σ k) s' (Build_state r' σ' k')⌝ ∗
+        ▷ |={∅,E}=> ∃ ρ', state_interp σ' ρ' ∗ stack_match ρ' r' k' ∗ wp E s' Q)%I.
 
 Local Instance wp_contractive : Contractive (wp_pre).
 Proof.
-  rewrite /wp_pre /= => n wp wp' Hwp F E s Q.
+  rewrite /wp_pre /= => n wp wp' Hwp E s Q.
   do 26 (f_contractive || f_equiv). apply Hwp.
 Qed.
 
 Local Definition wp_def := fixpoint wp_pre.
 Local Definition wp_aux : seal (@wp_def). Proof. by eexists. Qed.
-Definition wp_expr := wp_aux.(unseal).
-Local Lemma wp_unseal   : wp_expr = @wp_def.
+Definition wp := wp_aux.(unseal).
+Local Lemma wp_unseal   : wp = @wp_def.
 Proof. rewrite -wp_aux.(seal_eq) //. Qed.
 
+Lemma wp_unfold E s Q : wp E s Q ⊣⊢ wp_pre wp E s Q.
+Proof. rewrite wp_unseal. apply (fixpoint_unfold wp_pre). Qed.
 
 End wp.
