src/lifting_cont.v
@@ -5,6 +5,8 @@ Section wp.
 
 Context `{!gen_heapGS loc val Σ} `{!envGS val Σ} `{!invGS_gen HasNoLc Σ}.
 
+Variable (F : func_env).
+
 Fixpoint cont_to_stack k : env_state * nat :=
   match k with
   | Kstop => (∅, O)
@@ -12,18 +14,24 @@ Fixpoint cont_to_stack k : env_state * nat :=
   | Kseq _ k' | Kwhile _ _ k' => cont_to_stack k'
   end.
 
-Definition stack_match ρ r k := let '(ρ0, n) := cont_to_stack k in ρ = <[n := r]>ρ0.
+Definition stack_match ρ r k := assert_of (λ n, ⌜let '(ρ0, n0) := cont_to_stack k in n = n0 ∧ ρ = <[n := r]>ρ0⌝)%I.
 
-Definition wp_sk_pre (wp : func_env -d> coPset -d> stmt -d> cont -d> assert -d> assert) :
-    func_env -d> coPset -d> stmt -d> cont -d> assert -d> assert := λ F E s k Q,
+Lemma stack_env_match ρ r k : stack_match ρ r k ⊢ env_match ρ r.
+Proof.
+  split => n /=; apply bi.pure_mono.
+  destruct (cont_to_stack k); intros (_ & ->); by rewrite lookup_insert.
+Qed.
+
+Definition wp_sk_pre (wp : coPset -d> stmt -d> cont -d> assert -d> assert) :
+    coPset -d> stmt -d> cont -d> assert -d> assert := λ E s k Q,
  ((⌜s = Sskip ∧ k = Kstop⌝ ∗ |={E}=> Q) ∨
-  ∀ σ ρ, state_interp σ ρ ={E,∅}=∗ ∀ r, ⌜stack_match ρ r k⌝ -∗ ∃ s' r' σ' k',
+  ∀ σ ρ, state_interp σ ρ ={E,∅}=∗ ∀ r, stack_match ρ r k -∗ ∃ s' r' σ' k',
         ⌜step F s (Build_state r σ k) s' (Build_state r' σ' k')⌝ ∗
-        ▷ |={∅,E}=> ∃ ρ', state_interp σ' ρ' ∗ ⌜stack_match ρ' r' k'⌝ ∗ wp F E s' k' Q)%I.
+        ▷ |={∅,E}=> ∃ ρ', state_interp σ' ρ' ∗ stack_match ρ' r' k' ∗ wp E s' k' Q)%I.
 
 Local Instance wp_sk_pre_contractive : Contractive (wp_sk_pre).
 Proof.
-  rewrite /wp_sk_pre /= => n wp wp' Hwp F E s k Q.
+  rewrite /wp_sk_pre /= => n wp wp' Hwp E s k Q.
   do 25 (f_contractive || f_equiv); apply Hwp.
 Qed.
 
@@ -33,13 +41,64 @@ Definition wp_sk := wp_sk_aux.(unseal).
 Local Lemma wp_sk_unseal   : wp_sk = @wp_sk_def.
 Proof. rewrite -wp_sk_aux.(seal_eq) //. Qed.
 
+Lemma wp_sk_unfold E s k Q : wp_sk E s k Q ⊣⊢ wp_sk_pre wp_sk E s k Q.
+Proof. rewrite wp_sk_unseal. apply (fixpoint_unfold wp_sk_pre). Qed.
+
 Record postassert :=
   { Qnormal : assert; Qbreak : assert; Qcontinue : assert; Qreturn : val → assert }.
 
-Definition guarded F E Q k R :=
-  (Qnormal Q -∗ wp_sk F E Sskip k R) ∧
-  (Qbreak Q -∗ ∃ e s k', ⌜find_loop k = Some (Kwhile e s k')⌝ ∧ wp_sk F E Sskip k' R) ∧
-  (Qcontinue Q -∗ ∃ k', ⌜find_loop k = Some k'⌝ ∧ wp_sk F E Sskip k' R) ∧
-  (∀ e, wp_expr E e (Qreturn Q) -∗ ∃ k', ⌜find_call k = Some k'⌝ ∧ wp_sk F E (Sreturn e) k' R).
+Definition guarded E Q k R :=
+  ((Qnormal Q -∗ wp_sk E Sskip k R) ∧
+   (Qbreak Q -∗ ∃ e s k', ⌜find_loop k = Some (Kwhile e s k')⌝ ∧ wp_sk E Sskip k' R) ∧
+   (Qcontinue Q -∗ ∃ k', ⌜find_loop k = Some k'⌝ ∧ wp_sk E Sskip k' R) ∧
+   (∀ e, wp_expr E e (Qreturn Q) -∗ ∃ k', ⌜find_call k = Some k'⌝ ∧ wp_sk E (Sreturn e) k' R))%I.
+
+Definition wp E s Q := (∀ k R, guarded E Q k R -∗ wp_sk E s k R)%I.
+
+Print stmt.
+
+Lemma wp_skip E Q : Qnormal Q ⊢ wp E skip Q.
+Proof.
+  iIntros "H %% Hguard"; by iApply "Hguard".
+Qed.
+
+Lemma var_e : forall x v σ ρ r k, points_to_var x v ∗ state_interp σ ρ ∗ stack_match ρ r k ⊢ ⌜r !! x = Some v⌝.
+Proof.
+  intros; rewrite /state_interp; split => n; monPred.unseal.
+  iIntros "(Hx & (_ & Hρ) & Hmatch)".
+  iDestruct (var_e with "[$Hx $Hρ]") as %?.
+  destruct (cont_to_stack k) eqn: Hk; iDestruct "Hmatch" as %(<- & ->).
+  by rewrite /env_to_environ lookup_insert in H.
+Qed.
+
+Lemma var_update : forall x v v' σ ρ r k, points_to_var x v ∗ state_interp σ ρ ∗ stack_match ρ r k ⊢
+  |==> ∃ ρ', points_to_var x v' ∗ state_interp σ ρ' ∗ stack_match ρ' (<[x := v']>r) k.
+Proof.
+  intros; rewrite /state_interp; split => n; monPred.unseal.
+  iIntros "(Hx & ($ & Hρ) & Hmatch)".
+  iMod (var_update with "[$Hx $Hρ]") as "($ & $)".
+  iModIntro; iStopProof; apply bi.pure_mono.
+  destruct (cont_to_stack k) eqn: Hk; intros (<- & ->).
+  rewrite /set_var lookup_insert insert_insert //.
+Qed.
+
+Lemma wp_assign E x e Q : wp_expr E e (λ v, (∃ v0, points_to_var x v0) ∗
+  (points_to_var x v -∗ Qnormal Q)) ⊢ wp E (Sassign x e) Q.
+Proof.
+  iIntros "H %% Hguard".
+  rewrite wp_sk_unfold /wp_sk_pre; iRight.
+  iIntros (??) "S".
+  rewrite /wp_expr.
+  iMod ("H" with "S") as (?) "(He & S & (% & Hx) & Hpost)".
+  iApply fupd_mask_intro; first set_solver; iIntros "Hclose" (?) "Hstack".
+  iDestruct (var_e with "[$Hx $S $Hstack]") as %?.
+  iDestruct ("He" with "[Hstack]") as %?; first by iApply stack_env_match.
+  iExists skip, (<[x := v]>r), σ, k; iSplit.
+  { iPureIntro; by constructor. }
+  iNext.
+  iMod (var_update with "[$Hx $S $Hstack]") as (?) "(Hx & $ & $)".
+  iMod "Hclose"; iModIntro.
+  by iApply "Hguard"; iApply "Hpost".
+Qed.
 
 End wp.
