src/lifting_expr.v
@@ -9,6 +9,32 @@ Context `{!gen_heapGS loc val Σ} `{!envGS val Σ} `{!invGS_gen HasNoLc Σ}.
 
 Implicit Types (ρ : @env_state val) (σ : gmap loc val).
 
+Definition stack_level (n : nat) : assert := monPred_in(I := stack_index) n.
+
+Lemma stack_level_intro : ⊢ ∃ n, stack_level n.
+Proof.
+  by iDestruct (monPred_in_intro emp%I with "[]") as (?) "($ & _)".
+Qed.
+
+Lemma stack_level_elim : forall (P : assert) n, ⊢ stack_level n -∗ ⎡P n⎤ -∗ P.
+Proof.
+  intros; iIntros "#? H".
+  iApply bi.impl_elim_r; iSplit; first iApply "H".
+  by iApply monPred_in_elim.
+Qed.
+
+Lemma stack_level_embed : forall n (P : assert), ⊢ stack_level n -∗ P -∗ ⎡P n⎤.
+Proof.
+  split => ?; rewrite /stack_level; monPred.unseal.
+  iIntros "_" (? [=] [=] ? [=]); subst; auto.
+Qed.
+
+Lemma stack_level_eq : forall a b, ⊢ stack_level a -∗ stack_level b -∗ ⌜a = b⌝.
+Proof.
+  split => n; rewrite /stack_level; monPred.unseal; simpl.
+  iIntros; iPureIntro; congruence.
+Qed.
+
 Definition state_interp σ ρ : assert := (⎡gen_heap_interp σ⎤ ∗ ⎡env_auth ρ⎤)%I.
 
 Definition env_match ρ r := assert_of (λ n, ⌜ρ !! n = Some r⌝)%I.
@@ -17,7 +43,5 @@ Definition wp_expr E e Q : assert :=
   (∀ σ ρ, state_interp σ ρ ={E}=∗
      ∃ v, (∀ r, env_match ρ r -∗ ⌜eval_expr e r σ v⌝) ∗
           state_interp σ ρ ∗ Q v)%I.
-
-
 
 End wp_expr.
